src/basicmodal/semantics/completeness.lean
@@ -1,9 +1,9 @@
-import basicmodal.semantics.consistency
+import basicmodal.semantics.consistency basicmodal.syntax.soundness
 local attribute [instance] classical.prop_decidable
 
 open prfK
-
 namespace canonical
+
 
 def canonical (AX : ctx) [hax : sem_cons AX] : frame := 
 { 
@@ -11,13 +11,26 @@ def canonical (AX : ctx) [hax : sem_cons AX] : frame :=
   h := begin have h1 := max_ax_exists AX hax, choose Γ h1 using h1, exact ⟨⟨Γ, h1⟩⟩ end,
   rel := λ xΓ yΔ, ∀ φ : form, □φ ∈ xΓ.val → φ ∈ yΔ.val
 }
-#check canonical
+
 
 def val_canonical (AX : ctx) [hax : sem_cons AX] : nat → (canonical AX).states → Prop :=
   λ n, λ xΓ : (canonical AX).states, (p n) ∈ xΓ.val
 
+
 lemma existence (AX : ctx) (hax : sem_cons AX) (xΓ : (canonical AX).states) :
-  ∀ φ, ◇φ ∈ xΓ.val → ∃ yΔ : (canonical AX).states, φ ∈ yΔ.val ∧ (canonical AX).rel xΓ yΔ := sorry
+  ∀ φ, ◇φ ∈ xΓ.val → ∃ yΔ : (canonical AX).states, φ ∈ yΔ.val ∧ (canonical AX).rel xΓ yΔ :=
+begin
+simp, intros φ h1,
+let Γbox : ctx := {ψ : form | □ψ ∈ xΓ.val},
+have h1 : ax_consist AX (Γbox ∪ φ), by_contradiction h2,
+have h3 : ∃ L', (∀ ψ ∈ L', ψ ∈ Γbox) ∧ prfK AX (fin_conj L' ⊃ ¬φ), 
+  from five AX Γbox φ h2,
+cases h3 with L h3, cases h3 with h3 h4,
+have h5 : prfK AX (□(fin_conj L ⊃ ¬φ)), from nec h4,
+have h6 : prfK AX (□(fin_conj L) ⊃ □(¬φ)), from mp kdist h5,
+simp at *, sorry, simp at *, sorry
+end
+
 
 lemma truth (AX : ctx) (hax : sem_cons AX) (xΓ : (canonical AX).states) : 
   ∀ φ, forces (canonical AX) (val_canonical AX) xΓ φ ↔ (φ ∈ xΓ.val) :=
@@ -34,20 +47,48 @@ specialize ih_ψ_mp h2, sorry,
 intro h1, split, repeat {sorry}
 end
 
-theorem completeness (K : ctx) (φ : form) : sem_csq K φ → prfK K φ :=
+lemma comphelper (AX : ctx) (φ : form) (hax : sem_cons AX) : 
+  ¬ prfK AX φ → ax_consist AX {¬φ} :=
+begin
+intro h1, rw ax_consist, intros L h2,
+rw fin_ax_consist, simp at *,
+induction L, rw fin_conj, simp, by_contradiction h3,
+have h4 : prfK AX ⊥, from mp dne h3,
+have h5 : ¬prfK AX ⊥, from nprfalse AX hax,
+exact absurd h4 h5, 
+simp at *, 
+cases h2 with h2 h3, subst h2,
+specialize L_ih h3, rw fin_conj,
+sorry
+end 
+
+theorem completeness (hax : sem_cons ∅) (φ : form) : 
+  global_sem_csq ∅ φ → prfK ∅ φ :=
 begin
 rw ←not_imp_not, intro h1,
-have h2 : ax_consist K {¬φ}, 
-{simp at *, rw ax_consist, intros L h2, rw fin_ax_consist,
-have h3 : L = [¬φ], simp at *, sorry,
-subst h3, simp at *, rw fin_conj, rw fin_conj, simp at *, 
-have h4 : prfK K ((¬(¬φ)) ⊃ (¬(¬φ)&¬⊥)), sorry,
-have h6 : prfK K (φ ⊃ (¬(¬φ)&¬⊥)), simp at *,
-sorry, sorry},
-have h3 : ∃ Γ', max_ax_consist K Γ' ∧ {¬φ} ⊆ Γ', from lindenbaum K {¬φ} h2,
+have h2 : ax_consist ∅ {¬φ}, from comphelper ∅ φ hax h1,
+have h3 : ∃ Γ', max_ax_consist ∅ Γ' ∧ {¬φ} ⊆ Γ', from lindenbaum ∅ {¬φ} h2,
+simp at *, cases h3 with Γ' h3, cases h3 with h3 h4, 
+rw global_sem_csq, rw not_forall, let f := canonical, use f ∅,
+rw not_forall, let v := val_canonical, use v ∅, rw not_forall,
+let xΓ' : (f ∅).states := ⟨Γ', h3⟩, use xΓ', 
+rw not_imp, split,
+intros y ψ h5, 
+have h6 : ψ ∉ ∅, {exact set.not_mem_empty ψ},
+exact absurd h5 h6,
+have h5 : forces (f ∅) (v ∅) xΓ' (¬φ) ↔ ((¬φ) ∈ xΓ'.val), 
+  from truth ∅ hax xΓ' ¬φ,
 simp at *,
-cases h3 with Γ' h3, cases h3 with h3 h4, sorry
+cases h5 with h5 h6,
+have h7 : ¬forces (f ∅) (v ∅) xΓ' φ ↔ forces (f ∅) (v ∅) xΓ' ¬φ, 
+  from not_forces_imp (f ∅) (v ∅) xΓ' φ,
+simp at *, cases h7 with h7 h8, apply h8, apply h6, exact h4,
 end
 
-
 end canonical
+
+theorem T_completeness (φ : form) : F_valid φ ref_class → prfK T_axioms φ := sorry
+
+theorem S4_completeness (φ : form) : F_valid φ ref_trans_class → prfK S4_axioms φ := sorry
+
+theorem S5_completeness (φ : form) : F_valid φ equiv_class → prfK S5_axioms φ := sorry
